theories/typing/programs.v
@@ -615,7 +615,7 @@ Section typing.
     find_in_context (FindLoc l) T.
   Proof. iDestruct 1 as (β ty) "[Hl HT]". iExists (_, _) => /=. iFrame. Qed.
   Global Instance find_in_context_type_loc_id_inst l :
-    FindInContext (FindLoc l) 0%nat FICSyntactic :=
+    FindInContext (FindLoc l) FICSyntactic | 1 :=
     λ T, i2p (find_in_context_type_loc_id l T).
 
   Lemma find_in_context_type_val_id v T:
@@ -623,7 +623,7 @@ Section typing.
     find_in_context (FindVal v) T.
   Proof. iDestruct 1 as (ty) "[Hl HT]". iExists _ => /=. iFrame. Qed.
   Global Instance find_in_context_type_val_id_inst v :
-    FindInContext (FindVal v) 0%nat FICSyntactic :=
+    FindInContext (FindVal v) FICSyntactic | 1 :=
     λ T, i2p (find_in_context_type_val_id v T).
 
   Lemma find_in_context_type_val_P_id v T:
@@ -631,7 +631,7 @@ Section typing.
     find_in_context (FindValP v) T.
   Proof. iDestruct 1 as (ty) "[Hl HT]". iExists (ty_own_val ty _) => /=. iFrame. Qed.
   Global Instance find_in_context_type_val_P_id_inst v :
-    FindInContext (FindValP v) 0%nat FICSyntactic :=
+    FindInContext (FindValP v) FICSyntactic | 1 :=
     λ T, i2p (find_in_context_type_val_P_id v T).
 
   Lemma find_in_context_type_val_P_loc_id l T:
@@ -639,7 +639,7 @@ Section typing.
     find_in_context (FindValP l) T.
   Proof. iDestruct 1 as (β ty) "[Hl HT]". iExists (ty_own _ _ _) => /=. iFrame. Qed.
   Global Instance find_in_context_type_val_P_loc_id_inst (l : loc) :
-    FindInContext (FindValP l) 1%nat FICSyntactic :=
+    FindInContext (FindValP l) FICSyntactic | 10 :=
     λ T, i2p (find_in_context_type_val_P_loc_id l T).
 
   Lemma find_in_context_type_val_or_loc_P_id_val (v : val) (l : loc) T:
@@ -647,7 +647,7 @@ Section typing.
     find_in_context (FindValOrLoc v l) T.
   Proof. iDestruct 1 as (ty) "[Hl HT]". iExists (ty_own_val ty _) => /=. iFrame. Qed.
   Global Instance find_in_context_type_val_or_loc_P_id_val_inst v l:
-    FindInContext (FindValOrLoc v l) 0%nat FICSyntactic :=
+    FindInContext (FindValOrLoc v l) FICSyntactic | 1 :=
     λ T, i2p (find_in_context_type_val_or_loc_P_id_val v l T).
 
   Lemma find_in_context_type_val_or_loc_P_val_loc (lv l : loc) T:
@@ -655,7 +655,7 @@ Section typing.
     find_in_context (FindValOrLoc lv l) T.
   Proof. iDestruct 1 as (β ty) "[Hl HT]". iExists _. by iFrame. Qed.
   Global Instance find_in_context_type_val_or_loc_P_val_loc_inst (lv l : loc):
-    FindInContext (FindValOrLoc lv l) 1%nat FICSyntactic :=
+    FindInContext (FindValOrLoc lv l) FICSyntactic | 10 :=
     λ T, i2p (find_in_context_type_val_or_loc_P_val_loc lv l T).
 
   Lemma find_in_context_type_val_or_loc_P_id_loc (v : val) (l : loc) T:
@@ -663,7 +663,7 @@ Section typing.
     find_in_context (FindValOrLoc v l) T.
   Proof. iDestruct 1 as (β ty) "[Hl HT]". iExists (l ◁ₗ{β} ty)%I => /=. iFrame. Qed.
   Global Instance find_in_context_type_val_or_loc_P_id_loc_inst v l:
-    FindInContext (FindValOrLoc v l) 2%nat FICSyntactic :=
+    FindInContext (FindValOrLoc v l) FICSyntactic | 20 :=
     λ T, i2p (find_in_context_type_val_or_loc_P_id_loc v l T).
 
   Lemma find_in_context_loc_in_bounds l T :
@@ -671,7 +671,7 @@ Section typing.
     find_in_context (FindLocInBounds l) T.
   Proof. iDestruct 1 as (n) "[??]". iExists (loc_in_bounds _ _) => /=. iFrame. Qed.
   Global Instance find_in_context_loc_in_bounds_inst l :
-    FindInContext (FindLocInBounds l) 0 FICSyntactic :=
+    FindInContext (FindLocInBounds l) FICSyntactic | 1 :=
     λ T, i2p (find_in_context_loc_in_bounds l T).
 
   Lemma find_in_context_loc_in_bounds_loc l T :
@@ -679,7 +679,7 @@ Section typing.
     find_in_context (FindLocInBounds l) T.
   Proof. iDestruct 1 as (β ty) "[??]". iExists (ty_own _ _ _) => /=. iFrame. Qed.
   Global Instance find_in_context_loc_in_bounds_loc_inst l :
-    FindInContext (FindLocInBounds l) 1 FICSyntactic :=
+    FindInContext (FindLocInBounds l) FICSyntactic | 10 :=
     λ T, i2p (find_in_context_loc_in_bounds_loc l T).
 
   Lemma find_in_context_alloc_alive_global l T :
@@ -687,7 +687,7 @@ Section typing.
     find_in_context (FindAllocAlive l) T.
   Proof. iDestruct 1 as "?". iExists _ => /=. iFrame. Qed.
   Global Instance find_in_context_alloc_alive_global_inst l :
-    FindInContext (FindAllocAlive l) 0 FICSyntactic :=
+    FindInContext (FindAllocAlive l) FICSyntactic | 1 :=
     λ T, i2p (find_in_context_alloc_alive_global l T).
 
   Lemma find_in_context_alloc_alive_loc l T :
@@ -695,7 +695,7 @@ Section typing.
     find_in_context (FindAllocAlive l) T.
   Proof. iDestruct 1 as (β ty) "[??]". iExists (ty_own _ _ _) => /=. iFrame. Qed.
   Global Instance find_in_context_alloc_alive_loc_inst l :
-    FindInContext (FindAllocAlive l) 1 FICSyntactic :=
+    FindInContext (FindAllocAlive l) FICSyntactic | 10 :=
     λ T, i2p (find_in_context_alloc_alive_loc l T).
 
   Global Instance related_to_loc l β ty : RelatedTo (l ◁ₗ{β} ty)  | 100 := {| rt_fic := FindLoc l |}.
